ArkLib.lean
@@ -107,6 +107,8 @@ import ArkLib.Interaction.Boundary.Reification
 import ArkLib.Interaction.Boundary.Security
 import ArkLib.Interaction.Concurrent.Control
 import ArkLib.Interaction.Concurrent.Current
+import ArkLib.Interaction.Concurrent.Bisimulation
+import ArkLib.Interaction.Concurrent.Equivalence
 import ArkLib.Interaction.Concurrent.Examples
 import ArkLib.Interaction.Concurrent.Execution
 import ArkLib.Interaction.Concurrent.Fairness
